WIP: BDD

BDD/Basic.lean
@@ -1,1 +1,40 @@
-def hello := "world"
+import Std
+import Common.DDClasses
+
+inductive BDD where
+  | leaf (id' : Nat) (value : Bool)
+  | node (id' : Nat) (left right : BDD)
+deriving BEq, Hashable, Repr
+
+instance : Inhabited BDD where
+  default := .leaf 0 false
+
+def BDD.id (self : BDD) : Nat := match self with
+  | .leaf id' _ => id'
+  | .node id' _ _ => id'
+
+def BDD.low (self : BDD) : Option BDD := match self with
+  | .leaf _ _ => none
+  | .node _ left _ => some left
+
+def BDD.high (self : BDD) : Option BDD := match self with
+  | .leaf _ _ => none
+  | .node _ _ right => some right
+
+instance : DecisionDiagramTree BDD where
+  id := BDD.id
+--  newConstant : Bool → BDD := sorry
+--  addNewVar (index: Nat) (low high : BDD) : BDD := sorry
+--  isConstant : BDD → Bool := sorry
+--  unifiedKey : BDD → Nat := sorry
+--  index : BDD → Option Nat := sorry
+  low := BDD.low
+  high := BDD.high
+--  buildIndexer : BDD → Std.HashMap BDD Nat × Std.HashMap Nat BDD := sorry
+
+example : (default : BDD).id = 0 := rfl
+
+instance : ToString BDD where
+  toString := fun bdd => match bdd with
+    | .leaf id' value => s!"leaf {id'} {value}"
+    | .node id' left right => s!"node {id'} {left.id} {right.id}"
