Common/DDClasses.lean
@@ -1,15 +1,16 @@
 import Std.Data.HashMap
 
 class DecisionDiagramTree (α : Type) [BEq α] [Hashable α] where
-  len : α → Nat
-  newConstant : Bool → α
-  addNewVar (index: Nat) (low high : α) : α
-  isConstant : α → Bool
-  unifiedKey : α → Nat
-  index : α → Option Nat
+  id (self : α) : Nat
+--  len : α → Nat
+--  newConstant : Bool → α
+--  addNewVar (index: Nat) (low high : α) : α
+--  isConstant : α → Bool
+--  unifiedKey : α → Nat
+--  index : α → Option Nat
   low : α → Option α
   high : α → Option α
-  buildIndexer : α → Std.HashMap α Nat × Std.HashMap Nat α
+--  buildIndexer : α → Std.HashMap α Nat × Std.HashMap Nat α
 
 class ReducibleDecisionDiagramTree (α : Type) [BEq α] [Hashable α] extends DecisionDiagramTree α where
   reduce : α → α
